src/program_proof/lockservice/fmcounter_map.v
@@ -1,0 +1,63 @@
+From iris.algebra Require Import auth numbers gmap.
+From iris.proofmode Require Import base tactics classes.
+From iris.base_logic Require Import lib.own.
+From iris.bi.lib Require Import fractional.
+From Perennial.algebra Require Import fmcounter.
+From Perennial.goose_lang Require Import prelude.
+
+Class fmcounter_mapG Σ :=
+   { fmcounter_map_inG :> inG Σ (gmapUR u64 fmcounterUR) }.
+
+Section fmcounter_map_props.
+  Context `{!fmcounter_mapG Σ}.
+
+Definition fmcounter_map_own γ (k:u64) q n := own γ {[ k := (●{q}MaxNat n)]}.
+Definition fmcounter_map_lb γ (k:u64) n := own γ {[ k := (◯MaxNat n)]}.
+
+Notation "k fm[[ γ ]]↦{ q } n " := (fmcounter_map_own γ k q%Qp n)
+(at level 20, format "k fm[[ γ ]]↦{ q }  n") : bi_scope.
+Notation "k fm[[ γ ]]↦ n " := (k fm[[ γ ]]↦{ 1 } n)%I
+(at level 20, format "k fm[[ γ ]]↦ n") : bi_scope.
+Notation "k fm[[ γ ]]≥ n " := (fmcounter_map_lb γ k n)
+(at level 20, format "k fm[[ γ ]]≥ n") : bi_scope.
+Notation "k fm[[ γ ]]> n " := (fmcounter_map_lb γ k (n + 1))
+(at level 20, format "k fm[[ γ ]]> n") : bi_scope.
+
+Lemma fmcounter_map_get_lb γ k q n :
+      k fm[[γ]]↦{q} n ==∗ k fm[[γ]]↦{q} n ∗ k fm[[γ]]≥ n.
+Admitted.
+
+Lemma fmcounter_map_update γ k (n n':nat):
+  n ≤ n' ->
+      k fm[[γ]]↦ n ==∗ k fm[[γ]]↦ n'.
+Admitted.
+
+Lemma fmcounter_map_agree_lb γ k q n1 n2 :
+  k fm[[γ]]↦{q} n1 -∗ k fm[[γ]]≥ n2 -∗ ⌜n1 ≥ n2⌝.
+Admitted.
+
+Lemma fmcounter_map_agree_strict_lb γ k q n1 n2 :
+  k fm[[γ]]↦{q} n1 -∗ k fm[[γ]]> n2 -∗ ⌜n1 > n2⌝.
+Admitted.
+
+Lemma fmcounter_map_mono_lb (n1 n2:nat) γ k :
+  n1 ≤ n2 ->
+  k fm[[γ]]≥ n2 -∗ k fm[[γ]]≥ n1.
+Admitted.
+
+(* TODO: in the real fmcounter_map, this will need some preconditions *)
+Lemma fmcounter_map_alloc n γ k :
+  True
+  ==∗ k fm[[γ]]↦ n.
+Admitted.
+
+End fmcounter_map_props.
+
+Notation "k fm[[ γ ]]↦{ q } n " := (fmcounter_map_own γ k q%Qp n)
+(at level 20, format "k fm[[ γ ]]↦{ q }  n") : bi_scope.
+Notation "k fm[[ γ ]]↦ n " := (k fm[[ γ ]]↦{ 1 } n)%I
+(at level 20, format "k fm[[ γ ]]↦ n") : bi_scope.
+Notation "k fm[[ γ ]]≥ n " := (fmcounter_map_lb γ k n)
+(at level 20, format "k fm[[ γ ]]≥ n") : bi_scope.
+Notation "k fm[[ γ ]]> n " := (fmcounter_map_lb γ k (n + 1))
+(at level 20, format "k fm[[ γ ]]> n") : bi_scope.
