src/program_proof/lockservice/rpc.v
@@ -1,0 +1,149 @@
+From Perennial.program_proof.lockservice Require Import lockservice fmcounter_map.
+From iris.program_logic Require Export weakestpre.
+From Perennial.goose_lang Require Import prelude.
+From Perennial.goose_lang Require Import ffi.disk_prelude.
+From Perennial.goose_lang Require Import notation.
+From Perennial.program_proof Require Import proof_prelude.
+From stdpp Require Import gmap.
+From RecordUpdate Require Import RecordUpdate.
+From Perennial.algebra Require Import auth_map fmcounter.
+From Perennial.goose_lang.lib Require Import lock.
+From Perennial.Helpers Require Import NamedProps.
+From Perennial.Helpers Require Import ModArith.
+From iris.algebra Require Import numbers.
+From Coq.Structures Require Import OrdersTac.
+
+Section rpc.
+
+Class RPCRequest (A:Type) :=
+  { getCID : A -> u64 ;
+    getSeq : A -> u64
+  }.
+
+Context `{rpca : RPCRequest A ,
+          rpcr : R
+         }.
+
+Context `{!heapG Σ}.
+Context `{fmcounter_mapG Σ}.
+Context `{!inG Σ (exclR unitO)}.
+Context `{!mapG Σ (u64*u64) (option R)}.
+
+Record TryLockArgsC :=
+  mkTryLockArgsC{
+  Lockname:u64;
+  CID:u64;
+  Seq:u64
+  }.
+
+Record RPC_GS :=
+  mkγrpc {
+      rc:gname;
+      lseq:gname;
+      cseq:gname
+    }.
+
+Instance TryLockArgs_rpc : RPCRequest TryLockArgsC := {getCID x := x.(CID); getSeq x := x.(CID)}.
+
+Definition RPCRequest_inv (PreCond  : A -> iProp Σ) (PostCond  : A -> R -> iProp Σ) (args:A) (γrpc:RPC_GS) (γPost:gname) : iProp Σ :=
+   "#Hlseq_bound" ∷ args.(getCID) fm[[γrpc.(cseq)]]> int.nat args.(getSeq)
+  ∗ ("Hreply" ∷ (args.(getCID), args.(getSeq)) [[γrpc.(rc)]]↦ None ∗ PreCond args ∨
+      args.(getCID) fm[[γrpc.(lseq)]]≥ int.nat args.(getSeq)
+      ∗ (∃ (last_reply:R), (args.(getCID), args.(getSeq)) [[γrpc.(rc)]]↦ro Some last_reply
+        ∗ (own γPost (Excl ()) ∨ PostCond args last_reply)
+      )
+    ).
+
+Definition ReplyCache_inv (γrpc:RPC_GS) : iProp Σ :=
+  ∃ replyHistory:gmap (u64 * u64) (option R),
+      ("Hrcctx" ∷ map_ctx γrpc.(rc) 1 replyHistory)
+    ∗ ("#Hcseq_lb" ∷ [∗ map] cid_seq ↦ _ ∈ replyHistory, cid_seq.1 fm[[γrpc.(cseq)]]> int.nat cid_seq.2)
+.
+
+Definition replyCacheInvN : namespace := nroot .@ "replyCacheInvN".
+Definition rpcRequestInvN := nroot .@ "rpcRequestInvN".
+Lemma server_processes_request (PreCond  : A -> iProp Σ) (PostCond  : A -> R -> iProp Σ) (args:A) (old_seq:u64) (γrpc:RPC_GS) (reply:R)
+      (lastSeqM:gmap u64 u64) (lastReplyM:gmap u64 R) γP :
+     (int.val args.(getSeq) > int.val old_seq)%Z
+  -> (inv replyCacheInvN (ReplyCache_inv γrpc ))
+  -∗ (inv rpcRequestInvN (RPCRequest_inv PreCond PostCond args γrpc γP))
+  -∗ PostCond args reply
+  -∗ ([∗ map] cid↦seq ∈ <[args.(getCID):=old_seq]> lastSeqM, cid fm[[γrpc.(lseq)]]↦ int.nat seq)
+  -∗ ([∗ map] cid ↦ seq ; r ∈ lastSeqM ; lastReplyM, (cid, seq) [[γrpc.(rc)]]↦ro Some r)
+  ={⊤}=∗
+    (args.(getCID), args.(getSeq)) [[γrpc.(rc)]]↦ro Some reply
+  ∗ ([∗ map] cid↦seq ∈ <[args.(getCID):=args.(getSeq)]> lastSeqM, cid fm[[γrpc.(lseq)]]↦ int.nat seq)
+  ∗ ([∗ map] cid↦seq;y ∈ <[args.(getCID):=args.(getSeq)]> lastSeqM;
+                <[args.(getCID):=reply]> lastReplyM, 
+                (cid, seq) [[γrpc.(rc)]]↦ro Some y).
+Proof.
+  intros.
+  iIntros "Hlinv HargsInv Hpost Hlseq_own #Hrcagree".
+  iInv "HargsInv" as "[#>Hargseq_lb Hcases]" "HMClose".
+  iDestruct "Hcases" as "[[>Hunproc Hpre]|Hproc]".
+  {
+    iInv replyCacheInvN as ">HNinner" "HNClose".
+    iNamed "HNinner".
+    iDestruct (map_update _ _ (Some reply) with "Hrcctx Hunproc") as ">[Hrcctx Hrcptsto]".
+    iDestruct (map_freeze with "Hrcctx Hrcptsto") as ">[Hrcctx #Hrcptsoro]".
+    iDestruct (big_sepM_insert_2 _ _ (args.(getCID), args.(getSeq)) (Some reply) with "[Hargseq_lb] Hcseq_lb") as "Hcseq_lb2"; eauto.
+    iMod ("HNClose" with "[Hrcctx Hcseq_lb2]") as "_".
+    { iNext. iExists _; iFrame; iFrame "#". }
+
+    iDestruct (big_sepM_delete _ _ (args.(getCID)) _ with "Hlseq_own") as "[Hlseq_one Hlseq_own]"; first by apply lookup_insert.
+    iMod (fmcounter_map_update _ _ _ (int.nat args.(getSeq)) with "Hlseq_one") as "Hlseq_one"; first lia.
+    iMod (fmcounter_map_get_lb with "Hlseq_one") as "[Hlseq_one #Hlseq_new_lb]".
+    iDestruct (big_sepM_insert_delete with "[$Hlseq_own $Hlseq_one]") as "Hlseq_own".
+    rewrite ->insert_insert in *.
+    iMod ("HMClose" with "[Hpost]") as "_".
+    { iNext. iFrame "#". iRight. iFrame. iExists _; iFrame "#".
+      by iRight.
+    }
+    iModIntro.
+
+    iDestruct (big_sepM2_insert_2 _ lastSeqM lastReplyM args.(getCID) args.(getSeq) reply with "[Hargseq_lb] Hrcagree") as "Hrcagree2"; eauto.
+  }
+  { (* One-shot update of γrc already happened; this is impossible *)
+    iDestruct "Hproc" as "[#>Hlseq_lb _]".
+    iDestruct (big_sepM_delete _ _ (args.(getCID)) _ with "Hlseq_own") as "[Hlseq_one Hlseq_own]"; first by apply lookup_insert.
+    iDestruct (fmcounter_map_agree_lb with "Hlseq_one Hlseq_lb") as %Hlseq_lb_ineq.
+    iExFalso; iPureIntro.
+    replace (int.val old_seq) with (Z.of_nat (int.nat old_seq)) in H0; last by apply u64_Z_through_nat.
+    replace (int.val args.(getSeq)) with (Z.of_nat (int.nat args.(getSeq))) in Hlseq_lb_ineq; last by apply u64_Z_through_nat.
+    lia.
+  }
+Qed.
+
+Lemma smaller_seqno_stale_fact (args:A) (lseq:u64) (γrpc:RPC_GS) lastSeqM lastReplyM:
+  lastSeqM !! args.(getCID) = Some lseq ->
+  (int.val args.(getSeq) < int.val lseq)%Z ->
+  inv replyCacheInvN (ReplyCache_inv γrpc) -∗
+  ([∗ map] cid↦seq;r ∈ lastSeqM;lastReplyM, (cid, seq) [[γrpc.(rc)]]↦ro Some r)
+    ={⊤}=∗
+  args.(getCID) fm[[γrpc.(cseq)]]>(int.nat args.(getSeq) + 1).
+Proof.
+  intros.
+  iIntros "#Hinv #Hsepm".
+  iInv replyCacheInvN as ">HNinner" "HNclose".
+  iNamed "HNinner".
+  iDestruct (big_sepM2_dom with "Hsepm") as %Hdomeq.
+  assert (is_Some (lastReplyM !! args.(getCID))) as HlastReplyIn.
+  { apply elem_of_dom. assert (is_Some (lastSeqM !! args.(getCID))) by eauto. apply elem_of_dom in H2.
+    rewrite <- Hdomeq. done. }
+  destruct HlastReplyIn as [r HlastReplyIn].
+  iDestruct (big_sepM2_delete _ _ _ _ lseq r with "Hsepm") as "[Hptstoro _]"; eauto.
+  iDestruct (map_ro_valid with "Hrcctx Hptstoro") as %HinReplyHistory.
+  iDestruct (big_sepM_delete _ _ _ with "Hcseq_lb") as "[Hcseq_lb_one _] /="; eauto.
+  iDestruct (fmcounter_map_mono_lb (int.nat args.(getSeq) + 2) with "Hcseq_lb_one") as "#HStaleFact".
+  { replace (int.val args.(getSeq)) with (Z.of_nat (int.nat args.(getSeq))) in H1; last by apply u64_Z_through_nat.
+    replace (int.val lseq) with (Z.of_nat (int.nat lseq)) in H0; last by apply u64_Z_through_nat.
+    lia.
+  }
+  iMod ("HNclose" with "[Hrcctx]") as "_".
+  {
+    iNext. iExists _; iFrame; iFrame "#".
+  }
+  iModIntro. by replace (int.nat args.(getSeq) + 2) with (int.nat args.(getSeq) + 1 + 1) by lia.
+Qed.
+
+End rpc.
